FunMaps.v
@@ -31,17 +31,7 @@ Proof.
   contradiction.
 Qed.
 
-Section FunMaps_AbsR.
-
-Variables A B : Type.
-Variable R    : A -> B -> Prop.
-Variable or   : FunRel M.key A.
-Variable nr   : M.t B.
-Variable H    : SetMap_AbsR or nr R.
-
-Hypothesis Oeq_eq : forall a b, O.eq a b -> a = b.
-
-Ltac reduce :=
+Ltac reduction :=
   teardown; subst;
   try match goal with
   | [ H1 : SetMap_AbsR _ _ _,
@@ -64,11 +54,35 @@ Ltac reduce :=
     exists data
   end.
 
+Section FunMaps_AbsR.
+
+Variables A B : Type.
+Variable R    : A -> B -> Prop.
+Variable or   : FunRel M.key A.
+Variable nr   : M.t B.
+Variable H    : SetMap_AbsR or nr R.
+
+Hypothesis Oeq_eq : forall a b, O.eq a b -> a = b.
+
+Lemma Find_find_if P P' a b b' :
+  (forall i a b, R a b -> P i a <-> is_true (P' i b))
+    -> R b b'
+    -> Find P a b or <-> find_if P' nr = Some (a, b').
+Proof.
+  split; intros.
+    destruct H2.
+    eapply H0 in H3; eauto.
+    destruct (H a); clear H H5.
+    destruct (H4 _ H2); clear H2 H4.
+    destruct H; clear H.
+    unfold find_if.
+Abort.
+
 Lemma Update_SetMap_AbsR : forall k v v',
   R v v' -> SetMap_AbsR (Update k v or) (M.add k v' nr) R.
 Proof.
   split; intros.
-    reduce.
+    reduction.
       exists v'.
       split; trivial.
       apply F.find_mapsto_iff, F.add_mapsto_iff.
@@ -84,7 +98,7 @@ Proof.
     apply Oeq_eq in H1; subst.
     right; constructor.
   apply F.find_mapsto_iff in H2.
-  reduce; intuition.
+  reduction; intuition.
   left; constructor; auto.
   unfold Ensembles.In; simpl.
   unfold not; intros.
@@ -95,7 +109,7 @@ Lemma Remove_SetMap_AbsR : forall k,
   SetMap_AbsR (Remove k or) (M.remove k nr) R.
 Proof.
   split; intros.
-    reduce.
+    reduction.
     intuition.
     apply F.find_mapsto_iff, F.remove_mapsto_iff.
     split; auto.
@@ -104,7 +118,7 @@ Proof.
   apply F.find_mapsto_iff, F.remove_mapsto_iff in H0.
   destruct H0.
   apply F.find_mapsto_iff in H1.
-  reduce.
+  reduction.
   intuition.
   constructor; trivial.
   unfold Ensembles.In; simpl.
